added an extended assumption tactic

util/meta/tactic/basic.lean
@@ -57,4 +57,38 @@ end
 
 end
 
+meta def match_head (e : expr) : expr → tactic unit
+| e' :=
+    unify e e'
+<|> match e' with
+     | `(_ → %%e') :=
+     do v ← mk_mvar,
+        match_head (e'.instantiate_var v)
+     | _ := failed
+    end
+
+meta def find_matching_head : expr → list expr → tactic expr
+| e []         := failed
+| e (H :: Hs) :=
+  do t ← infer_type H,
+     (match_head e t >> return H) <|> find_matching_head e Hs
+
+meta def xassumption : tactic unit :=
+do { ctx ← local_context,
+     t   ← target,
+     H   ← find_matching_head t ctx,
+     tactic.apply H }
+<|> fail "assumption tactic failed"
+
+example {a b : Prop} (h₀ : a → b) (h₁ : a) : b :=
+begin
+  xassumption,
+  xassumption,
+end
+
+example {α : Type} {p : α → Prop} (h₀ : ∀ x, p x) (y : α) : p y :=
+begin
+  xassumption,
+end
+
 end tactic.interactive
